@prefix mud: <https://w3id.org/mud#> .
@prefix xsd: <http://www.w3.org/2001/XMLSchema#> .
@prefix rdf: <http://www.w3.org/1999/02/22-rdf-syntax-ns#> .
@prefix rdfs: <http://www.w3.org/2000/01/rdf-schema#> .
@prefix owl: <http://www.w3.org/2002/07/owl#> .

mud:Referencable a rdfs:Class
    ; rdfs:label "Referencable"
    ; rdfs:comment "A thing that can be referenced via auto-generated UUIDv5-hashed HMAC-SHA256 hashed UUID-URN-URIs or anonymously via local names or indexicals."
.

    mud:refHash a rdf:Property
        ; rdfs:domain mud:Referencable
        ; rdfs:range xsd:string
    .

    mud:ref a rdf:Property
        ; rdfs:domain mud:Referencable
        ; rdfs:range xsd:string
        ; rdfs:comment "A local name a user can use on his machine to reference a resource. These names are always rendered/skolemized to the UUIDv5 URI of the mud:refHash"
    .


mud:this a rdf:Property
    ; rdfs:domain mud:Referencable
    ; rdfs:comment "This property will be resolved by the precompiler to `a {class} ; mud:ref {lower-cased(class)}`"
    ; rdfs:comment "This property is intended to have RDFS classes as its range. However, to maintain compatibility with various OWL profiles, we deliberately omit a formal rdfs:range definition."
.

mud:I a owl:NamedIndividual
    ; rdfs:comment "This resource will be resolved by the precompiler to `[a og:Agent ; mud:ref \"agent\"]`"
.

